Update pcuic after functorisation of declarations typing

pcuic/theories/PCUICAst.v
@@ -122,7 +122,14 @@ Record mutual_inductive_entry := {
   Module PCUICTerm <: Term.
 
     Definition term := term.
+
+    Definition tRel := tRel.
     Definition tSort := tSort.
+    Definition tProd := tProd.
+    Definition tLetIn := tLetIn.
+    Definition tInd := tInd.
+
+    Definition mkApps := mkApps.
 
   End PCUICTerm.
 
